{
  "@context": {
    "rdf": "http://www.w3.org/1999/02/22-rdf-syntax-ns#",
    "rdfs": "http://www.w3.org/2000/01/rdf-schema#",
    "xsd": "http://www.w3.org/2001/XMLSchema#"
  },
  "@graph": [
                {
                    "@id": "https://[OTTO]/Participant",
                    "@type": "rdfs:Class",
                    "rdfs:comment": "A legal entity that can agree to federation policies.",
                    "rdfs:label": "Participant",
                    "rdfs:subClassOf":
                        {
                            "@id": "http://schema.org/Organization"
                        }
                },
                {
                    "@id": "https://[OTTO]/Federation",
                    "@type": "rdfs:Class",
                    "rdfs:comment": "An organization that defines common policies and operating procedures.",
                    "rdfs:label": "Federation",
                    "rdfs:subClassOf":
                        {
                            "@id": "http://schema.org/Organization"
                        }
                },
                {
                    "@id": "https://[OTTO]/RegistrationAuthority",
                    "@type": "rdfs:Class",
                    "rdfs:comment": "An organization that operates the technical infrastructure for federations.",
                    "rdfs:label": "RegistrationAuthority",
                    "rdfs:subClassOf":
                        {
                            "@id": "http://schema.org/Organization"
                        }
                },
                {
                    "@id": "https://[OTTO]/Entity",
                    "@type": "rdfs:Class",
                    "rdfs:comment": "A digital service operated by a Participant",
                    "rdfs:label": "Entity",
                    "rdfs:subClassOf":
                        {
                            "@id": "http://schema.org/Thing"
                        }
                },
                {
                    "@id": "https://[OTTO]/OpenIDProvider",
                    "@type": "rdfs:Class",
                    "rdfs:comment": "An implementation of the OpenID Connect Provider interfaces.",
                    "rdfs:label": "OpenIDProvider",
                    "rdfs:subClassOf":
                        {
                            "@id": "https://[OTTO]/Entity"
                        }
                },
                {
                    "@id": "https://[OTTO]/OpenIDRelyingParty",
                    "@type": "rdfs:Class",
                    "rdfs:comment": "An implementation of the OpenID Connect Relying Party interfaces.",
                    "rdfs:label": "OpenIDRelyingParty",
                    "rdfs:subClassOf":
                        {
                            "@id": "https://[OTTO]/Entity"
                        }
                },
                {
                    "@id": "https://[OTTO]/TrustMark",
                    "@type": "rdfs:Class",
                    "rdfs:comment": "A statement of conformance to a well-scoped set of identity trust and/or interoperability requirements.",
                    "rdfs:label": "TrustMark",
                    "rdfs:subClassOf":
                        {
                            "@id": "http://schema.org/Thing"
                        }
                },
                {
                    "@id": "https://[OTTO]/TrustMarkProvider",
                    "@type": "rdfs:Class",
                    "rdfs:comment": "An organization that issues trustmarks based on a formal assessment process.",
                    "rdfs:label": "TrustMarkProvider",
                    "rdfs:subClassOf":
                        {
                            "@id": "http://schema.org/Organization"
                        }
                },
                {
                    "@id": "https://[OTTO]/TrustMarkPolicy",
                    "@type": "rdfs:Class",
                    "rdfs:comment": "Set of rules under which the Trustmark was issued.",
                    "rdfs:label": "TrustMarkPolicy",
                    "rdfs:subClassOf":
                        {
                            "@id": "http://schema.org/DigitalDocument"
                        }
                },
                {
                    "@id": "https://[OTTO]/TrustMarkDefinition",
                    "@type": "rdfs:Class",
                    "rdfs:comment": "The formal assessment process for a trustmark.",
                    "rdfs:label": "TrustMarkDefinition",
                    "rdfs:subClassOf":
                        {
                            "@id": "http://schema.org/DigitalDocument"
                        }
                },
                {
                    "@id": "https://[OTTO]/TrustMarkAgreement",
                    "@type": "rdfs:Class",
                    "rdfs:comment": "The agreement signed the organization to which the trustmark was issued.",
                    "rdfs:label": "TrustMarkAgreement",
                    "rdfs:subClassOf":
                        {
                            "@id": "http://schema.org/DigitalDocument"
                        }
                },
                {
                    "@id": "https://[OTTO]/TrustMarkProfile",
                    "@type": "rdfs:Class",
                    "rdfs:comment": "a set of trustmarks that a Trustmark Recipient must possess, in order to meet the trust and interoperability requirements of Trustmark Relying Parties in that community.",
                    "rdfs:label": "TrustMarkProfile",
                    "rdfs:subClassOf":
                        {
                            "@id": "http://schema.org/Thing"
                        }
                },
                {
                  "@id": "http://schema.org/operates",
                  "@type": "rdf:Property",
                  "http://schema.org/domainIncludes": [
                    {
                      "@id": "https://[OTTO]/Participant"
                    }
                  ],
                  "http://schema.org/rangeIncludes": {"@id": "http://[OTTO]/Entity"},
                  "rdfs:comment": "Service provided by the Participant",
                  "rdfs:label": "operates"
                },

  ]
  "@id": "http://kantarainitive.com/otto/1.0"
}
