                {
                    "@id": "https://[OTTO]/TrustMark",
                    "@type": "rdfs:Class",
                    "rdfs:comment": "A statement of conformance to a well-scoped set of identity trust and/or interoperability requirements.",
                    "rdfs:label": "TrustMark",
                    "rdfs:subClassOf":
                        {
                            "@id": "http://schema.org/Thing"
                        }
                },
                {
                    "@id": "https://[OTTO]/TrustMarkProvider",
                    "@type": "rdfs:Class",
                    "rdfs:comment": "An organization that issues trustmarks based on a formal assessment process.",
                    "rdfs:label": "TrustMarkProvider",
                    "rdfs:subClassOf":
                        {
                            "@id": "http://schema.org/Organization"
                        }
                },
                {
                    "@id": "https://[OTTO]/TrustMarkPolicy",
                    "@type": "rdfs:Class",
                    "rdfs:comment": "Set of rules under which the Trustmark was issued.",
                    "rdfs:label": "TrustMarkPolicy",
                    "rdfs:subClassOf":
                        {
                            "@id": "http://schema.org/DigitalDocument"
                        }
                },
                {
                    "@id": "https://[OTTO]/TrustMarkDefinition",
                    "@type": "rdfs:Class",
                    "rdfs:comment": "The formal assessment process for a trustmark.",
                    "rdfs:label": "TrustMarkDefinition",
                    "rdfs:subClassOf":
                        {
                            "@id": "http://schema.org/DigitalDocument"
                        }
                },
                {
                    "@id": "https://[OTTO]/TrustMarkAgreement",
                    "@type": "rdfs:Class",
                    "rdfs:comment": "The agreement signed the organization to which the trustmark was issued.",
                    "rdfs:label": "TrustMarkAgreement",
                    "rdfs:subClassOf":
                        {
                            "@id": "http://schema.org/DigitalDocument"
                        }
                },
                {
                    "@id": "https://[OTTO]/TrustMarkProfile",
                    "@type": "rdfs:Class",
                    "rdfs:comment": "a set of trustmarks that a Trustmark Recipient must possess, in order to meet the trust and interoperability requirements of Trustmark Relying Parties in that community.",
                    "rdfs:label": "TrustMarkProfile",
                    "rdfs:subClassOf":
                        {
                            "@id": "http://schema.org/Thing"
                        }
                },

